proved some things about the types, and added lots of automation

src/wacket.v
@@ -39,16 +39,24 @@ Notation "'(' 'Bool' b ')'" := (D_Boolean b).
 Notation "'(' 'Prim1' op exp ')'" := (D_UniOp op exp).
 Notation "'(' 'If' b 'Then' t 'Else' e ')'" := (D_if b t e).
 
-Inductive typ: Type :=
-| typ_Int
-| typ_Bool
-| typ_Error
+Inductive dupeType: Type :=
+| D_type_Int
+| D_type_Bool
+| D_type_Error
 .
 
-Definition typeToString (t:typ) : string := match t with 
-| typ_Int => "Int"
-| typ_Bool => "Bool"
-| typ_Error => "Error"
+Definition typeSame t1 t2 := match (t1,t2) with 
+| (D_type_Int,D_type_Int) => true
+| (D_type_Bool,D_type_Bool) => true
+| (D_type_Error,D_type_Error) => true
+| _ => false
+end.
+
+
+Definition typeToString (t:dupeType) : string := match t with 
+| D_type_Int => "Int"
+| D_type_Bool => "Bool"
+| D_type_Error => "Error"
 end.
 
 Inductive dupeResult : Type :=
@@ -58,26 +66,46 @@ Inductive dupeResult : Type :=
 .
 
 Definition resultType result := match result with 
-| DR_Int _ => typ_Int
-| DR_Bool _ => typ_Bool
-| DR_Error => typ_Error
+| DR_Int _ => D_type_Int
+| DR_Bool _ => D_type_Bool
+| DR_Error => D_type_Error
 end.
 
-Definition uniOpExpectedType op := match op with 
-| D_U_add1 => typ_Int
-| D_U_sub1 => typ_Int
-| D_U_zero => typ_Int
-| D_U_not => typ_Bool
+Definition uniOpTypeSignature op := match op with 
+| D_U_add1 => (D_type_Int,D_type_Int)::nil
+| D_U_sub1 => (D_type_Int,D_type_Int)::nil
+| D_U_zero => (D_type_Int,D_type_Bool)::nil
+| D_U_not => (D_type_Bool,D_type_Bool)::nil
 end. 
 
-Definition uniOpResultType op := match op with 
-| D_U_add1 => typ_Int
-| D_U_sub1 => typ_Int
-| D_U_zero => typ_Bool
-| D_U_not => typ_Bool
-end. 
+Definition uniOpAcceptsType op typ := 
+    let (accepts,returns) := split (uniOpTypeSignature op) in
+    In typ accepts
+. 
 
-Definition UniOpTransform op result := match (op, result) with 
+
+
+Definition uniOpTypeSignatureForAccept op t := 
+    let signatureList := uniOpTypeSignature op in 
+    let fix search lst := match lst with 
+    | (accepts,returns)::tail => if typeSame accepts t 
+            then Some (accepts,returns)
+            else search tail 
+    | nil => None
+    end in search signatureList
+.
+
+Definition uniOpTypeSignatureForReturn op t := 
+    let signatureList := uniOpTypeSignature op in 
+    let fix search lst := match lst with 
+    | (accepts,returns)::tail => if typeSame returns t 
+            then Some (accepts,returns)
+            else search tail 
+    | nil => None
+    end in search signatureList
+.
+
+Definition uniOpTransform op result := match (op, result) with 
 | (D_U_add1, DR_Int z) => DR_Int (z + 1)
 | (D_U_sub1, DR_Int z) => DR_Int (z - 1)
 | (D_U_zero, DR_Int z) => DR_Bool (z =? 0)
@@ -85,40 +113,305 @@ Definition UniOpTransform op result := match (op, result) with
 | _ => DR_Error
 end.
 
+
 Fixpoint evalDupe(d : dupe) := match d with 
 | (D_Integer z) => (DR_Int z)
 | (D_Boolean b) => (DR_Bool b)
-| D_UniOp op exp => UniOpTransform op (evalDupe exp)
-| (D_if e1 e2 e3) => match (evalDupe e1) with 
-    | DR_Int i => evalDupe e2
-    | DR_Bool b => if b then evalDupe e2  else evalDupe e3 
-    | DR_Error => DR_Error
+| (D_UniOp op exp) => uniOpTransform op (evalDupe exp)
+| (D_if e1 e2 e3) => match (evalDupe e1, evalDupe e2, evalDupe e3) with 
+    | (DR_Bool b, res1, res2) => 
+        if (typeSame (resultType res1) (resultType res2)) && (negb (typeSame (resultType res1) D_type_Error))
+        then if b then res1 else res2
+        else DR_Error
+    | (DR_Int _, res1, res2 ) =>
+        if (typeSame (resultType res1) (resultType res2)) && (negb (typeSame (resultType res1) D_type_Error))
+        then res1
+        else DR_Error
+    | _ => DR_Error
     end
 end.
 
 
 (* this will probably have to be changed because of how integers are represented in binary*)
-Reserved Notation " t 'd==>' n " (at level 50, left associativity).
-Inductive dupeEval: dupe -> dupeResult -> Prop :=
-| E_D_Interger: forall z, (D_Integer z) d==> (DR_Int z)
-| E_D_Boolean: forall b, (D_Boolean b) d==> (DR_Bool b)
+Reserved Notation " src 'd==>' val " (at level 50, left associativity).
+Inductive dupeEval: dupe -> (dupeType * dupeResult)%type -> Prop :=
+| E_D_Interger: forall z, (D_Integer z) d==> (D_type_Int, (DR_Int z))
+| E_D_Boolean: forall b, (D_Boolean b) d==> (D_type_Bool ,(DR_Bool b))
 
-| E_D_UniOp: forall t v op,
-    t d==> v ->
-    (resultType v) = (uniOpExpectedType op) ->
-    (D_UniOp op t) d==> (UniOpTransform op v)
+| E_D_UniOp: forall t v inputType op evalType,
+    t d==> (inputType, v) ->
+    In (inputType, evalType) (uniOpTypeSignature op) ->
+    (D_UniOp op t) d==> (evalType,(uniOpTransform op v))
 
-| E_D_ifFalse: forall t_if t_then t_else v,
-    t_if d==> (DR_Bool false) -> 
-    t_else d==> v ->
-    (D_if t_if t_then t_else) d==> v
-| E_D_ifTrue: forall t_if t_then v t_else ,
-    t_if d==> (DR_Bool true) -> 
-    t_then d==> v ->
-    (D_if t_if t_then t_else) d==> v
-| E_D_ifInt: forall t_if z t_then v t_else ,
-    t_if d==> (DR_Int z) -> 
-    t_then d==> v ->
-    (D_if t_if t_then t_else) d==> v
+| E_D_ifFalse: forall t_if t_then vt t_else ve evalType,
+    t_if d==> (D_type_Bool,(DR_Bool false)) -> 
+    t_then d==> (evalType,vt) ->
+    t_else d==> (evalType,ve) ->
+    (D_if t_if t_then t_else) d==> (evalType,ve)
+| E_D_ifTrue: forall t_if t_then vt t_else ve evalType,
+    t_if d==> (D_type_Bool,(DR_Bool true)) -> 
+    t_then d==> (evalType,vt) ->
+    t_else d==> (evalType,ve) ->
+    (D_if t_if t_then t_else) d==> (evalType,vt)
+| E_D_ifInt: forall t_if z t_then vt t_else ve evalType,
+    t_if d==> (D_type_Int,(DR_Int z)) -> 
+    t_then d==> (evalType,vt) ->
+    t_else d==> (evalType,ve) ->
+    (D_if t_if t_then t_else) d==> (evalType,vt)
 
-where " t 'd==>' n " := (dupeEval t n).
+where " src 'd==>' val " := (dupeEval src val).
+
+
+Theorem evalTypesSame:
+    forall src val type,
+        src d==> (type, val) ->
+        resultType val = type.
+Proof.
+    induction src; intros;
+    destruct val; destruct type; (try reflexivity); simpl in *;
+    try (solve [inversion H]);
+    try (
+        destruct d; inversion H; subst; destruct H5; inversion H0; subst;
+        (eapply (IHsrc v) in H3);
+        destruct v
+    );
+    try (discriminate);
+    try (solve [inversion H; subst; 
+                eapply IHsrc3 in H7; eapply IHsrc2 in H6; 
+                (try discriminate)
+        ]).
+Qed.
+
+Ltac copyHypothesis H := 
+    let tmp := fresh "H" in 
+    let eq := fresh "eq" in
+    remember H as tmp eqn: eq; clear eq
+.
+
+Ltac rewriteLeft := match goal with 
+| H: ?l = _ |- context[?l] => rewrite -> H
+| H: ?l = _, H0: context[?l] |- _ => rewrite -> H in H0
+| _ => fail
+end.
+Ltac rewriteRight := match goal with 
+| H: _ = ?r |- context[?r] => rewrite <- H
+| H: _ = ?r, H0: context[?r] |- _ => rewrite <- H in H0
+| _ => fail
+end.
+
+
+Ltac specializeIH := match goal with 
+| IH: ?hyp -> ?prop, H: ?hyp |- _ => specialize (IH H)
+
+| H: ?src d==> (?type, ?val),
+    IH: forall val : dupeResult, 
+    ?src d==> (resultType val, val) -> evalDupe ?src = val |- _ =>
+
+    let tmp := fresh "H" in 
+    let eq := fresh "eq" in
+    remember H as tmp eqn: eq; clear eq;
+    specialize (IH val);
+    eapply evalTypesSame in tmp; rewrite tmp in IH;
+    specialize (IH H);
+    clear tmp
+
+| IH: forall val: dupeResult,
+    evalDupe ?src = val -> _ |- _ => specialize (IH (evalDupe src))
+
+| IH: ?a = ?a -> _ |- _ => 
+    let tmp := fresh "H" in 
+    assert (a = a) as tmp;[reflexivity | (specialize (IH tmp));clear tmp]
+
+| IH: (?t1 <> ?t2) -> _ |-  _ => 
+    let tmp := fresh "H" in 
+    assert (t1 <> t2) as tmp;[
+        solve[discriminate]|
+        specialize (IH tmp); clear tmp
+    ]
+end.
+
+
+Ltac solveUniOp := 
+    (repeat specializeIH);
+    repeat (
+        (try assumption);
+        (try discriminate);
+        (try contradiction);
+        (try reflexivity);
+        match goal with 
+        | dUniop: dupeUniaryOp, dResult: dupeResult |- _ => 
+            destruct dUniop; destruct dResult; simpl in *;
+            (try discriminate)
+        | H: uniOpTransform ?op (evalDupe ?src) = ?val |- (D_UniOp ?op ?src) d==> (_,?val) =>
+            rewrite <- H
+        | |- (D_UniOp ?op ?src) d==> (?type, uniOpTransform ?op ?srcResult) => 
+            apply (E_D_UniOp src srcResult (resultType srcResult) op type)
+        | H: uniOpTransform ?op ?srcVal = ?val |- In (resultType ?srcVal, ?resType) (uniOpTypeSignature ?op) => 
+            destruct srcVal; solve[(try discriminate H); (try contradiction); repeat ((left; reflexivity) || right)]
+        | IH: resultType ?srcResult <> D_type_Error -> _,
+            H0: uniOpTransform ?op ?srcResult = ?result |- _ => 
+            destruct srcResult; (try discriminate H0); simpl in IH
+        | IH: ?t1 <> ?t2 -> _ |-  _ => 
+            let tmp := fresh "H" in
+            assert (t1 <> t2) as tmp; [
+                solve[discriminate]|
+                specialize (IH tmp); clear tmp
+            ]
+        | H: ?val1 = ?val2 |- uniOpTransform ?op ?val1 = uniOpTransform ?op ?val2 =>
+            rewrite H
+        | H : _ \/ _ |- _ => destruct H
+        | H : _ /\ _ |- _ => destruct H
+        | H: ?l = _ |- context[?l] => rewrite -> H
+        | H: ?l = _, H0: context[?l] |- _ => rewrite -> H in H0
+        | _ => idtac "fail";fail
+        end
+    ).
+
+Ltac solveIfs := repeat (match goal with 
+| H: dupeResult |- _ => destruct H
+| |- evalDupe (D_if ?src1 ?src2 ?src3) = _ => simpl
+end); try match goal with 
+| H: D_if ?src1 ?src2 ?src3 d==> (_,_) |- _ => inversion H;subst
+end;
+repeat specializeIH;
+repeat (
+(try discriminate);
+(try contradiction);
+(try reflexivity);
+match goal with 
+| H: evalDupe (D_if ?src1 ?src2 ?src3) = _ |- _ => 
+    simpl in H; destruct (evalDupe src1); 
+    destruct (evalDupe src2); destruct (evalDupe src3);
+    simpl in *
+| IH: (?t1 <> ?t2) -> _ |-  _ => 
+    let tmp := fresh "H" in 
+    assert (t1 <> t2) as tmp;[
+        solve[discriminate]|
+        specialize (IH tmp); clear tmp
+    ]
+| H: context[if ?b then _ else _] |- _ => destruct b
+| H: ?l = _ |- context[?l] => rewrite -> H
+| H: ?l = _, H0: context[?l] |- _ => rewrite -> H in H0
+| Hsrc1: ?src1 d==> (D_type_Int, DR_Int ?z),
+    Hsrc2: ?src2 d==> (?evalType, ?valThen),
+    Hsrc3: ?src3 d==> (?evalType, ?valElse)
+    |- (D_if ?src1 ?src2 ?src3) d==> (?evalType, ?valThen) => 
+        apply (E_D_ifInt src1 z src2 valThen src3 valElse evalType); assumption
+| Hsrc1: ?src1 d==> (D_type_Bool, DR_Bool true),
+    Hsrc2: ?src2 d==> (?evalType, ?valThen),
+    Hsrc3: ?src3 d==> (?evalType, ?valElse)
+    |- (D_if ?src1 ?src2 ?src3) d==> (?evalType, ?valThen) => 
+        apply (E_D_ifTrue src1 src2 valThen src3 valElse evalType); assumption
+| Hsrc1: ?src1 d==> (D_type_Bool, DR_Bool false),
+    Hsrc2: ?src2 d==> (?evalType, ?valThen),
+    Hsrc3: ?src3 d==> (?evalType, ?valElse)
+    |- (D_if ?src1 ?src2 ?src3) d==> (?evalType, ?valElse) => 
+        apply (E_D_ifFalse src1 src2 valThen src3 valElse evalType); assumption
+| H: ?src d==> (?type, ?value) |- context[typeSame (resultType ?value) ?type] =>
+    let new := fresh "H" in 
+    let eq := fresh "eq" in
+    remember H as new eqn: eq; clear eq;
+    apply evalTypesSame in new;
+    rewrite new
+| H: ?src d==> (?type, ?value) |- context[typeSame ?type (resultType ?value)] =>
+    let new := fresh "H" in 
+    let eq := fresh "eq" in
+    remember H as new eqn: eq; clear eq;
+    apply evalTypesSame in new;
+    rewrite new
+end
+).
+
+
+
+
+Theorem evalDupe_implies_dupeEval: 
+    forall src val,
+    evalDupe src = val ->
+    ((resultType val) <> D_type_Error) ->
+    src d==> (resultType val, val).
+Proof.
+    induction src; intros;
+    try (simpl in *; subst; constructor).
+    - solveUniOp.
+    - solveIfs.
+Qed.
+
+
+
+
+Theorem dupeEval_implies_evalDupe: 
+    forall src val,
+    src d==> (resultType val, val) ->
+    evalDupe src = val.
+Proof.
+    induction src; intros; (try (inversion H; subst; reflexivity)).
+    - inversion H; subst. solveUniOp.
+    - solveIfs.
+Qed.
+
+Theorem dupeNotEvalError:
+forall src val,
+    src d==> (resultType val, val) ->
+    ((resultType val) <> D_type_Error).
+Proof.
+    induction src; intros;
+    try (inversion H; subst; discriminate).
+    - solveUniOp.
+    - repeat (match goal with 
+    | H: dupeResult |- _ => destruct H
+    | |- evalDupe (D_if ?src1 ?src2 ?src3) = _ => simpl
+    end).
+    try match goal with 
+    | H: D_if ?src1 ?src2 ?src3 d==> (_,_) |- _ => inversion H;subst
+    end.
+    repeat specializeIH.
+    repeat (
+    (try discriminate);
+    (try contradiction);
+    (try reflexivity);
+    match goal with 
+    | H: evalDupe (D_if ?src1 ?src2 ?src3) = _ |- _ => 
+        simpl in H; destruct (evalDupe src1); 
+        destruct (evalDupe src2); destruct (evalDupe src3);
+        simpl in *
+    | IH: (?t1 <> ?t2) -> _ |-  _ => 
+        let tmp := fresh "H" in 
+        assert (t1 <> t2) as tmp;[
+            solve[discriminate]|
+            specialize (IH tmp); clear tmp
+        ]
+    | H: context[if ?b then _ else _] |- _ => destruct b
+    | H: ?l = _ |- context[?l] => rewrite -> H
+    | H: ?l = _, H0: context[?l] |- _ => rewrite -> H in H0
+    | Hsrc1: ?src1 d==> (D_type_Int, DR_Int ?z),
+        Hsrc2: ?src2 d==> (?evalType, ?valThen),
+        Hsrc3: ?src3 d==> (?evalType, ?valElse)
+        |- (D_if ?src1 ?src2 ?src3) d==> (?evalType, ?valThen) => 
+            apply (E_D_ifInt src1 z src2 valThen src3 valElse evalType); assumption
+    | Hsrc1: ?src1 d==> (D_type_Bool, DR_Bool true),
+        Hsrc2: ?src2 d==> (?evalType, ?valThen),
+        Hsrc3: ?src3 d==> (?evalType, ?valElse)
+        |- (D_if ?src1 ?src2 ?src3) d==> (?evalType, ?valThen) => 
+            apply (E_D_ifTrue src1 src2 valThen src3 valElse evalType); assumption
+    | Hsrc1: ?src1 d==> (D_type_Bool, DR_Bool false),
+        Hsrc2: ?src2 d==> (?evalType, ?valThen),
+        Hsrc3: ?src3 d==> (?evalType, ?valElse)
+        |- (D_if ?src1 ?src2 ?src3) d==> (?evalType, ?valElse) => 
+            apply (E_D_ifFalse src1 src2 valThen src3 valElse evalType); assumption
+    | H: ?src d==> (?type, ?value) |- context[typeSame (resultType ?value) ?type] =>
+        let new := fresh "H" in 
+        let eq := fresh "eq" in
+        remember H as new eqn: eq; clear eq;
+        apply evalTypesSame in new;
+        rewrite new
+    | H: ?src d==> (?type, ?value) |- context[typeSame ?type (resultType ?value)] =>
+        let new := fresh "H" in 
+        let eq := fresh "eq" in
+        remember H as new eqn: eq; clear eq;
+        apply evalTypesSame in new;
+        rewrite new
+    end
+    ). 
+    
+        
